Fix build (I broke everything when trying to git merge)

backend/Tailcallproof.v
@@ -428,10 +428,10 @@ We first define the simulation invariant between call stacks.
 The first two cases are standard, but the third case corresponds
 to a frame that was eliminated by the transformation. *)
 
-Inductive match_stackframes (m: mem): compartment -> list stackframe -> list stackframe -> Prop :=
-  | match_stackframes_nil: forall cp,
+Inductive match_stackframes (m: mem) (cp: compartment): list stackframe -> list stackframe -> Prop :=
+  | match_stackframes_nil:
       match_stackframes m cp nil nil
-  | match_stackframes_normal: forall stk stk' res sp pc rs rs' ce f cp,
+  | match_stackframes_normal: forall stk stk' res sp pc rs rs' ce f,
       match_stackframes m (comp_of f) stk stk' ->
       forall (COMPAT: cenv_compat prog ce),
       forall (UPD: uptodate_caller (comp_of f) (call_comp stk) (call_comp stk')),
@@ -441,25 +441,13 @@ Inductive match_stackframes (m: mem): compartment -> list stackframe -> list sta
         (Stackframe res f (Vptr sp Ptrofs.zero) pc rs :: stk)
         (Stackframe res (transf_function ce f) (Vptr sp Ptrofs.zero) pc rs' :: stk')
   | match_stackframes_tail: forall stk stk' res sp pc rs f,
-      match_stackframes m (comp_of f) stk stk' ->
+      match_stackframes m cp stk stk' ->
       is_return_spec f pc res ->
       f.(fn_stacksize) = 0 ->
-      match_stackframes m (comp_of f)
+      cp = comp_of f ->
+      match_stackframes m cp
         (Stackframe res f (Vptr sp Ptrofs.zero) pc rs :: stk)
         stk'.
-
-(* Lemma match_stackframes_call_comp: forall m cp stk stk', *)
-(*     match_stackframes m cp stk stk' -> *)
-(*     (call_comp stk <> cp -> call_comp stk = call_comp stk'). *)
-(*     (* call_comp stk = call_comp stk'. *) *)
-(* Proof. *)
-(*   induction 1. *)
-(*   - reflexivity. *)
-(*   - simpl; rewrite comp_transf_function; reflexivity. *)
-(*   - simpl. intros. congruence. *)
-(*     (* specialize (IHmatch_stackframes H2). congruence. *) *)
-(* Qed. *)
-
 
 (** Here is the invariant relating two states.  The first three
   cases are standard.  Note the ``less defined than'' conditions
@@ -491,8 +479,8 @@ Inductive match_states: state -> state -> Prop :=
       match_stackframes m' cp s s' ->
       Val.lessdef v v' ->
       Mem.extends m m' ->
-      match_states (Returnstate s v m)
-                   (Returnstate s' v' m')
+      match_states (Returnstate s v m cp)
+                   (Returnstate s' v' m' cp)
   | match_states_interm:
       forall s sp pc rs m s' m' f r v'
              (STACKS: match_stackframes m' (comp_of f) s s')
@@ -501,29 +489,7 @@ Inductive match_states: state -> state -> Prop :=
       f.(fn_stacksize) = 0 ->
       Val.lessdef (rs#r) v' ->
       match_states (State s f (Vptr sp Ptrofs.zero) pc rs m)
-                   (Returnstate s' v' m')
-  | match_states_state_fail: forall s s' f sp pc rs m m' r v',
-      match_stackframes m' (comp_of f) s s' ->
-      forall (EXT: Mem.extends m m'),
-      is_return_spec f pc r ->
-      f.(fn_stacksize) = 0 ->
-      forall (LD: Val.lessdef (rs # r) v'),
-      Genv.type_of_call ge (call_comp s') (comp_of f) = Genv.CrossCompartmentCall ->
-      not (not_ptr v') ->
-      match_states (State s f (Vptr sp Ptrofs.zero) pc rs m)
-                   (Failstate s' v')
-  | match_states_return_fail: forall s cp s' v v' m m',
-      match_stackframes m' cp s s' ->
-      forall (EXT: Mem.extends m m'),
-      forall (LD: Val.lessdef v v'),
-      (Genv.type_of_call ge (call_comp s) cp = Genv.CrossCompartmentCall -> not_ptr v) ->
-      Genv.type_of_call ge (call_comp s') cp = Genv.CrossCompartmentCall ->
-      not (not_ptr v') ->
-      match_states (Returnstate s v m)
-                   (Failstate s' v')
-  | match_states_fail: forall s v s',
-      match_states (Failstate s v) s'.
-
+                   (Returnstate s' v' m' (comp_of f)).
 
 (** The last case of [match_states] corresponds to the execution
   of a move/nop/return sequence in the original code that was
@@ -546,8 +512,7 @@ Definition measure (st: state) : nat :=
   match st with
   | State s f sp pc rs m => (List.length s * (niter + 2) + return_measure f.(fn_code) pc + 1)%nat
   | Callstate s f args m => 0%nat
-  | Returnstate s v m => (List.length s * (niter + 2))%nat
-  | Failstate _ _ => 0%nat
+  | Returnstate s v m cp => (List.length s * (niter + 2))%nat
   end.
 
 Ltac TransfInstr :=
@@ -577,11 +542,7 @@ Proof.
 - (* nop *)
   TransfInstr. left. econstructor; split.
   eapply exec_Inop; eauto. constructor; auto.
-- (* eliminated nop success *)
-  assert (s0 = pc') by congruence. subst s0.
-  right. split. simpl. omega. split. auto.
-  econstructor; eauto.
-- (* eliminated nop fail *)
+- (* eliminated nop *)
   assert (s0 = pc') by congruence. subst s0.
   right. split. simpl. omega. split. auto.
   econstructor; eauto.
@@ -595,15 +556,10 @@ Proof.
   eapply exec_Iop; eauto.  rewrite <- EVAL'.
   apply eval_operation_preserved. exact symbols_preserved.
   econstructor; eauto. apply set_reg_lessdef; auto.
-- (* eliminated move success *)
+- (* eliminated move *)
   rewrite H1 in H. clear H1. inv H.
   right. split. simpl. omega. split. auto.
   econstructor; eauto. simpl in H0. rewrite PMap.gss. congruence.
-- (* eliminated move fail *)
-  rewrite H1 in H. clear H1. inv H.
-  right. split. simpl. omega. split. auto.
-  econstructor; eauto.
-  rewrite Regmap.gss. simpl in H0; congruence.
 
 - (* load *)
   TransfInstr.
@@ -667,17 +623,15 @@ Proof.
   eapply find_function_ptr_translated; eauto.
   rewrite comp_transl. eapply allowed_call_translated; eauto.
   rewrite comp_transl; eauto.
-  constructor. rewrite Efd.
-  eapply match_stackframes_tail; eauto.
+  constructor. eapply match_stackframes_tail; eauto.
   (* TODO: Should be a lemma? *)
-  { (* rewrite Efd. *)
+  { rewrite Efd.
     clear -FREE STACKS.
     revert STACKS. generalize (comp_of f). intros cp STACKS.
     induction STACKS.
     - constructor.
     - constructor; auto. eapply Mem.free_can_access_block_inj_1; eauto.
     - constructor; auto. }
-  unfold intra_compartment_call in INTRA.
     apply (cenv_compat_linkorder _ _ _ ORDER (compenv_program_compat _)).
   { red. simpl. congruence. }
   apply regs_lessdef_regs; auto.
@@ -726,9 +680,9 @@ Proof.
   rewrite comp_transl. eapply allowed_call_translated; eauto.
   rewrite stacksize_preserved; auto.
   rewrite comp_transl; eauto.
-  constructor. rewrite COMP.
+  constructor.
   (* TODO: Should be a lemma? *)
-  { clear -FREE STACKS.
+  { rewrite COMP. clear -FREE STACKS.
     revert STACKS. generalize (comp_of f). intros cp STACKS.
     induction STACKS.
     - constructor.
@@ -776,97 +730,35 @@ Proof.
   constructor; auto.
 
 - (* return *)
-  (* case analysis*)
-  Require Import Classical.
-  destruct (classic (Genv.type_of_call tge (call_comp s') (comp_of f) = Genv.CrossCompartmentCall ->
-                     not_ptr (regmap_optget or Vundef rs'))).
-+ exploit Mem.free_parallel_extends; eauto. intros [m'1 [FREE EXT]].
+  exploit Mem.free_parallel_extends; eauto. intros [m'1 [FREE EXT]].
   TransfInstr.
-  left. exists (Returnstate s' (regmap_optget or Vundef rs') m'1); split.
+  left. exists (Returnstate s' (regmap_optget or Vundef rs') m'1 (comp_of (transf_function ce f))); split.
   eapply exec_Ireturn; eauto.
-  rewrite stacksize_preserved, comp_transl; eauto. eauto.
-  rewrite comp_transf_function. eauto.
-  econstructor. instantiate (1 := comp_of f).
-  (* (* rewrite comp_transf_function. *) constructor. *)
+  rewrite stacksize_preserved, comp_transl; eauto.
+  rewrite comp_transf_function. constructor.
   (* TODO: Should be a lemma? *)
   { clear -FREE STACKS.
     revert STACKS. generalize (comp_of f). intros cp STACKS.
     induction STACKS.
     - constructor.
-    - constructor; eauto. eapply Mem.free_can_access_block_inj_1; eauto.
+    - constructor; auto. eapply Mem.free_can_access_block_inj_1; eauto.
     - constructor; auto. }
   destruct or; simpl. apply RLD. constructor.
   auto.
-+ exploit Mem.free_parallel_extends; eauto. intros [m'1 [FREE EXT]].
-  TransfInstr.
-  left. exists (Failstate s' (regmap_optget or Vundef rs')). split.
-  econstructor; eauto.
-  rewrite stacksize_preserved, comp_transl; eauto.
-  rewrite comp_transf_function. tauto.
-  econstructor. instantiate (1 := comp_of f). instantiate (1 := m'1).
-  { clear -FREE STACKS.
-    revert STACKS. generalize (comp_of f). intros cp STACKS.
-    induction STACKS.
-    - constructor.
-    - constructor; eauto. eapply Mem.free_can_access_block_inj_1; eauto.
-    - constructor; auto. }
-  eauto.
-  destruct or; simpl. apply RLD. constructor.
-  tauto. tauto. tauto.
 
-- (* eliminated return None success *)
+- (* eliminated return None *)
   assert (or = None) by congruence. subst or.
   right. split. simpl. omega. split. auto.
-  econstructor. eauto.
+  constructor. auto.
   simpl. constructor.
   eapply Mem.free_left_extends; eauto.
 
-- (* eliminated return Some success *)
+- (* eliminated return Some *)
   assert (or = Some r) by congruence. subst or.
   right. split. simpl. omega. split. auto.
-  econstructor. eauto.
+  constructor. auto.
   simpl. auto.
   eapply Mem.free_left_extends; eauto.
-
-- (* eliminated return None fail *)
-  assert (or = None) by congruence. subst or.
-  right. split. simpl. omega. split. auto.
-  econstructor. instantiate (1 := comp_of f). instantiate (1 := m'0).
-  eauto.
-  eapply Mem.free_left_extends; eauto.
-  now simpl.
-  tauto.
-  auto. auto.
-
-- (* eliminated return Some fail *)
-  assert (or = Some r) by congruence. subst or.
-  right. split. simpl. omega. split. auto.
-  econstructor. instantiate (1 := comp_of f). instantiate (1 := m'0).
-  eauto.
-  eapply Mem.free_left_extends; eauto.
-  auto.
-  tauto.
-  auto. auto.
-
-- right. split. simpl. omega.
-  split. reflexivity.
-  constructor.
-
-- right. split. simpl. omega.
-  split. reflexivity.
-  constructor.
-
-- right. split. simpl. omega.
-  split. reflexivity.
-  constructor.
-
-- right. split. simpl. omega.
-  split. reflexivity.
-  constructor.
-
-- right. split. simpl. omega.
-  split. reflexivity.
-  constructor.
 
 - (* internal call *)
   exploit Mem.alloc_extends; eauto.
@@ -896,15 +788,13 @@ Proof.
 - (* external call *)
   exploit external_call_mem_extends; eauto.
   intros [res' [m2' [A [B [C D]]]]].
-  destruct (classic (Genv.type_of_call tge (call_comp s') (comp_of ef) = Genv.CrossCompartmentCall ->
-                     not_ptr res')).
-+ left. exists (Returnstate s' res' m2'); split.
+  left. exists (Returnstate s' res' m2' (comp_of ef)); split.
   simpl. econstructor; eauto.
   eapply external_call_symbols_preserved; eauto. apply senv_preserved.
   destruct (needs_calling_comp (comp_of ef)) eqn:ALLOWED.
   { now rewrite <- (UPD ALLOWED). }
   exploit external_call_caller_independent; eauto.
-  econstructor; eauto. instantiate (1 := comp_of ef).
+  constructor; auto.
   (* TODO: Should be a lemma? *)
   { clear -A H5.
     remember (call_comp s) as cp. clear Heqcp. unfold comp_of in H5; simpl in H5.
@@ -912,50 +802,15 @@ Proof.
     - constructor.
     - constructor; auto. eapply external_call_can_access_block; eauto.
     - constructor; auto. }
-+ left. exists (Failstate s' res'). split.
-  econstructor; eauto.
-  eapply external_call_symbols_preserved; eauto. apply senv_preserved.
-  (* destruct (needs_calling_comp (comp_of ef)) eqn:ALLOWED. *)
-  (* { now rewrite <- (UPD ALLOWED). } *)
-  exploit external_call_caller_independent; eauto.
-  tauto.
-  econstructor. instantiate (1 := comp_of ef). instantiate (1 := m2').
-  { clear -A H5.
-    remember (call_comp s) as cp. clear Heqcp. unfold comp_of in H5; simpl in H5.
-    induction H5.
-    - constructor.
-    - constructor; auto. eapply external_call_can_access_block; eauto.
-    - constructor; auto. }
-  eauto.
-  auto.
-  tauto.
-  tauto.
-  auto.
-
-- exploit external_call_mem_extends; eauto.
-  intros [res' [m2' [A [B [C D]]]]].
-  destruct (classic (Genv.type_of_call tge (call_comp s') (comp_of ef) = Genv.CrossCompartmentCall ->
-                     not_ptr res')).
-  + left. exists (Returnstate s' res' m2'); split.
-    simpl. econstructor; eauto.
-    eapply external_call_symbols_preserved; eauto. apply senv_preserved.
-    destruct (needs_calling_comp (comp_of ef)) eqn:ALLOWED.
-    { now rewrite <- (UPD ALLOWED). }
-    exploit external_call_caller_independent; eauto.
-    econstructor; eauto.
-  + left. exists (Failstate s' res'). split.
-    econstructor.
-    eapply external_call_symbols_preserved; eauto. apply senv_preserved.
-    exploit external_call_caller_independent; eauto.
-    tauto.
-    auto.
-    constructor.
 
 - (* returnstate *)
-  inv H2.
+  inv H4.
 + (* synchronous return in both programs *)
   left. econstructor; split.
   apply exec_return.
+  rewrite comp_transf_function, <- type_of_call_translated.
+  { intros G. specialize (NO_CROSS_PTR G).
+    inv H5; auto; contradiction. }
   constructor; auto. apply set_reg_lessdef; auto.
 + (* return instr in source program, eliminated because of tailcall *)
   right. split. unfold measure. simpl length.
@@ -965,17 +820,6 @@ Proof.
   split. auto.
   econstructor; eauto.
   rewrite Regmap.gss. auto.
-
-- right. simpl. split.
-  generalize (return_measure_bounds (fn_code f) pc). unfold niter.
-  omega.
-  split. reflexivity.
-  inv H2.
-  + simpl in H5. rewrite comp_transf_function in H5.
-    simpl in H3. apply H3 in H5. exfalso. clear -H6 H5 LD.
-    inv LD; auto.
-  + econstructor; eauto.
-    rewrite Regmap.gss. auto.
 Qed.
 
 Lemma transf_initial_states:
@@ -1002,8 +846,7 @@ Lemma transf_final_states:
   forall st1 st2 r,
   match_states st1 st2 -> final_state st1 r -> final_state st2 r.
 Proof.
-  intros. inv H0. inv H. inv H5. inv H3. constructor.
-  inv LD; auto. simpl in H7. contradiction.
+  intros. inv H0. inv H. inv H5. inv H6. constructor.
 Qed.
 
 
